intuitionism

Cslib/Logics/Propositional/NaturalDeduction/Intuitionistic.lean
@@ -8,6 +8,20 @@ module
 public import Cslib.Logics.Propositional.NaturalDeduction.Basic
 public import Mathlib.Order.WithBot
 
+/-! # Intuitionistic PL
+
+This file introduces intuitionistic propositions (having a primitive falsum), and derivations
+(including the "falsum elimination" rule ex falso quodlibet). These definitions match the existing
+encodings of intuitionistic logic in minimal logic as follows:
+- `propEquiv : Proposition (WithBot Atom) ≃ IProposition Atom` : intuitionistic propositions can be
+  recovered by adjoining a bottom element to the atom type.
+- `ITheory.IDerivation.toDerivation` : every intuitionistic derivation can be turned into a minimal
+  one by adding efq to the collection of axioms.
+- `Theory.Derivation.toIDerivation` : any minimal derivation in the "intuitionistic completion" of
+  a theory (obtained by adding a bottom element and efq) can be turned into an intuitionistic
+  derivation.
+-/
+
 @[expose] public section
 
 universe u
@@ -16,76 +30,173 @@ namespace Cslib.Logic.PL
 
 open Proposition Theory Derivation InferenceSystem DerivableIn
 
-variable {Atom : Type u} [DecidableEq Atom] [Bot Atom]
+variable {Atom : Type u} [DecidableEq Atom]
+
+inductive IProposition (Atom : Type u) : Type u where
+  | atom (x : Atom) : IProposition Atom
+  | or (A B : IProposition Atom) : IProposition Atom
+  | and (A B : IProposition Atom) : IProposition Atom
+  | impl (A B : IProposition Atom) : IProposition Atom
+  | bot : IProposition Atom
+  deriving DecidableEq
+
+open IProposition
+
+instance : Bot (IProposition Atom) := ⟨.bot⟩
+
+/-- We view negation as a defined connective ~A := A → ⊥ -/
+abbrev IProposition.neg [Bot Atom] : IProposition Atom → IProposition Atom :=
+  (IProposition.impl · ⊥)
+
+/-- A fixed choice of a derivable Iproposition (of course any two are equivalent). -/
+abbrev IProposition.top : IProposition Atom := impl ⊥ ⊥
+
+instance instTopIProposition : Top (IProposition Atom) := ⟨.top⟩
+
+scoped infix:36 " ∧ " => IProposition.and
+scoped infix:35 " ∨ " => IProposition.or
+scoped infix:30 " → " => IProposition.impl
+scoped prefix:40 " ¬ " => IProposition.neg
+
+/-- Contexts are finsets of propositions. -/
+abbrev ICtx (Atom) := Finset (IProposition Atom)
+
+/-- Theories are sets of propositions. -/
+abbrev ITheory (Atom) := Set (IProposition Atom)
+
+open IProposition
 
 /-- An intuitionistic `T`-derivation of {A₁, ..., Aₙ} ⊢ B demonstrates B using (undischarged)
 assumptions among Aᵢ, possibly appealing to axioms from `T`. This adds ex falso quodlibet to
 `T`.Derivation. -/
-inductive Theory.IntDerivation {T : Theory Atom} : Ctx Atom → Proposition Atom → Type u where
+inductive ITheory.IDerivation {T : ITheory Atom} : ICtx Atom → IProposition Atom → Type u where
   /-- Axiom -/
-  | ax {Γ : Ctx Atom} {A : Proposition Atom} (_ : A ∈ T) : IntDerivation Γ A
+  | ax {Γ : ICtx Atom} {A : IProposition Atom} (_ : A ∈ T) : IDerivation Γ A
   /-- Assumption -/
-  | ass {Γ : Ctx Atom} {A : Proposition Atom} (_ : A ∈ Γ) : IntDerivation Γ A
+  | ass {Γ : ICtx Atom} {A : IProposition Atom} (_ : A ∈ Γ) : IDerivation Γ A
   /-- Conjunction introduction -/
-  | conjI {Γ : Ctx Atom} {A B : Proposition Atom} :
-      IntDerivation Γ A → IntDerivation Γ B → IntDerivation Γ (A ∧ B)
+  | conjI {Γ : ICtx Atom} {A B : IProposition Atom} :
+      IDerivation Γ A → IDerivation Γ B → IDerivation Γ (A ∧ B)
   /-- Conjunction elimination left -/
-  | conjE₁ {Γ : Ctx Atom} {A B : Proposition Atom} : IntDerivation Γ (A ∧ B) → IntDerivation Γ A
+  | conjE₁ {Γ : ICtx Atom} {A B : IProposition Atom} : IDerivation Γ (A ∧ B) → IDerivation Γ A
   /-- Conjunction elimination right -/
-  | conjE₂ {Γ : Ctx Atom} {A B : Proposition Atom} : IntDerivation Γ (A ∧ B) → IntDerivation Γ B
+  | conjE₂ {Γ : ICtx Atom} {A B : IProposition Atom} : IDerivation Γ (A ∧ B) → IDerivation Γ B
   /-- Disjunction introduction left -/
-  | disjI₁ {Γ : Ctx Atom} {A B : Proposition Atom} : IntDerivation Γ A → IntDerivation Γ (A ∨ B)
+  | disjI₁ {Γ : ICtx Atom} {A B : IProposition Atom} : IDerivation Γ A → IDerivation Γ (A ∨ B)
   /-- Disjunction introduction right -/
-  | disjI₂ {Γ : Ctx Atom} {A B : Proposition Atom} : IntDerivation Γ B → IntDerivation Γ (A ∨ B)
+  | disjI₂ {Γ : ICtx Atom} {A B : IProposition Atom} : IDerivation Γ B → IDerivation Γ (A ∨ B)
   /-- Disjunction elimination -/
-  | disjE {Γ : Ctx Atom} {A B C : Proposition Atom} : IntDerivation Γ (A ∨ B) →
-      IntDerivation (insert A Γ) C → IntDerivation (insert B Γ) C → IntDerivation Γ C
+  | disjE {Γ : ICtx Atom} {A B C : IProposition Atom} : IDerivation Γ (A ∨ B) →
+      IDerivation (insert A Γ) C → IDerivation (insert B Γ) C → IDerivation Γ C
   /-- Implication introduction -/
-  | implI {A B : Proposition Atom} (Γ : Ctx Atom) :
-      IntDerivation (insert A Γ) B → IntDerivation Γ (A → B)
+  | implI {A B : IProposition Atom} (Γ : ICtx Atom) :
+      IDerivation (insert A Γ) B → IDerivation Γ (A → B)
   /-- Implication elimination -/
-  | implE {Γ : Ctx Atom} {A B : Proposition Atom} :
-      IntDerivation Γ (A → B) → IntDerivation Γ A → IntDerivation Γ B
+  | implE {Γ : ICtx Atom} {A B : IProposition Atom} :
+      IDerivation Γ (A → B) → IDerivation Γ A → IDerivation Γ B
   /-- Ex falso quodlibet. -/
-  | efq {Γ : Ctx Atom} (A : Proposition Atom) : IntDerivation Γ ⊥ → IntDerivation Γ A
+  | efq {Γ : ICtx Atom} (A : IProposition Atom) : IDerivation Γ ⊥ → IDerivation Γ A
 
-variable {T : Theory Atom}
+open ITheory IDerivation
 
-def Theory.IntDerivation.toDerivation {T : Theory Atom} {Γ : Ctx Atom} {A : Proposition Atom} :
-    T.IntDerivation Γ A → (T ∪ IPL).Derivation Γ A
-  | ax hA => .ax (Set.mem_union_left IPL hA)
-  | ass hA => .ass hA
-  | conjI DA DB => .conjI DA.toDerivation DB.toDerivation
-  | conjE₁ D => .conjE₁ D.toDerivation
-  | conjE₂ D => .conjE₂ D.toDerivation
-  | disjI₁ D => .disjI₁ D.toDerivation
-  | disjI₂ D => .disjI₂ D.toDerivation
-  | disjE D DA DB => .disjE D.toDerivation DA.toDerivation DB.toDerivation
-  | implI Γ D => .implI Γ D.toDerivation
+/-- Minimal to intuitionistic. -/
+def Proposition.toIProposition : Proposition (WithBot Atom) → IProposition Atom
+  | atom ⊥ => ⊥
+  | atom (some x) => .atom x
+  | and A B => A.toIProposition ∧ B.toIProposition
+  | or A B => A.toIProposition ∨ B.toIProposition
+  | impl A B => A.toIProposition → B.toIProposition
+
+/-- Intuitionistic to minimal. -/
+def IProposition.toProposition : IProposition Atom → Proposition (WithBot Atom)
+  | atom x => .atom x
+  | and A B => A.toProposition ∧ B.toProposition
+  | or A B => A.toProposition ∨ B.toProposition
+  | impl A B => A.toProposition → B.toProposition
+  | bot => ⊥
+
+/-- Equivalence of encoded with genuine intuitionistic propositions. -/
+def propEquiv : Proposition (WithBot Atom) ≃ IProposition Atom where
+  toFun := Proposition.toIProposition
+  invFun := IProposition.toProposition
+  left_inv A := by
+    induction A
+    case atom x => cases x <;> rfl
+    all_goals simp_all [toIProposition, toProposition]
+  right_inv A := by
+    induction A
+    all_goals simp_all [toIProposition, toProposition]
+    rfl
+
+/-- Map contexts along `Proposition.toIProposition`. -/
+def Ctx.toICtx : Ctx (WithBot Atom) → ICtx Atom := Finset.image toIProposition
+
+@[simp] lemma Ctx.toICtx_insert (A : Proposition (WithBot Atom)) (Γ : Ctx (WithBot Atom)) :
+    (insert A Γ).toICtx = insert A.toIProposition Γ.toICtx := by simp [toICtx]
+
+/-- Map contexts along `IProposition.toProposition`. -/
+def ICtx.toCtx : ICtx Atom → Ctx (WithBot Atom) := Finset.image toProposition
+
+@[simp] lemma ICtx.toCtx_insert (A : IProposition Atom) (Γ : ICtx Atom) :
+    (insert A Γ).toCtx = insert A.toProposition Γ.toCtx := by simp [toCtx]
+
+/-- Map theories along `Proposition.toIProposition`. -/
+def Theory.toITheory (T : Theory Atom) : ITheory Atom :=
+  toIProposition ∘ (WithBot.some <$> ·) '' T
+
+/-- Map theories along `IProposition.toProposition`. -/
+def ITheory.toTheory (T : ITheory Atom) : Theory (WithBot Atom) :=
+  toProposition '' T ∪ IPL (WithBot Atom)
+
+/-- Intuitionistic completion of a theory. -/
+def Theory.iCompletion (T : Theory Atom) : Theory (WithBot Atom) :=
+  WithBot.some <$> T ∪ IPL (WithBot Atom)
+
+omit [DecidableEq Atom] in
+lemma Theory.toTheory_toITheory (T : Theory Atom) : T.toITheory.toTheory = T.iCompletion := by
+  have toTo (A : Proposition (WithBot Atom)) : A.toIProposition.toProposition = A :=
+    propEquiv.left_inv A
+  ext
+  simp [toTheory, toITheory, iCompletion, Functor.map, toTo]
+
+/-- Turn an intuitionistic derivation into a minimal one. -/
+def ITheory.IDerivation.toDerivation {T : ITheory Atom} {Γ : ICtx Atom} {A : IProposition Atom} :
+    (T.IDerivation Γ A) → (T.toTheory.Derivation Γ.toCtx A.toProposition)
+  | ax hA => .ax <| Set.mem_union_left _ ⟨A, hA, rfl⟩
+  | ass hA => .ass <| Finset.mem_image.mpr ⟨A, hA, rfl⟩
+  | conjI DA DB => .andI DA.toDerivation DB.toDerivation
+  | conjE₁ D => .andE₁ D.toDerivation
+  | conjE₂ D => .andE₂ D.toDerivation
+  | disjI₁ D => .orI₁ D.toDerivation
+  | disjI₂ D => .orI₂ D.toDerivation
+  | disjE D DA DB => .orE D.toDerivation
+    (Γ.toCtx_insert _ ▸ DA.toDerivation) (Γ.toCtx_insert _ ▸ DB.toDerivation)
+  | implI Γ D => .implI Γ.toCtx (Γ.toCtx_insert _ ▸ D.toDerivation)
   | implE D D' => .implE D.toDerivation D'.toDerivation
-  | efq A D => .implE (A := ⊥) (.ax (Set.mem_union_right T ⟨A, rfl⟩)) D.toDerivation
+  | efq A D => .implE (A := ⊥) (.ax (Set.mem_union_right _ ⟨A.toProposition, rfl⟩)) D.toDerivation
 
-theorem derivableIn_intuitionisticCompletion_iff_nonempty_intDerivation {T : Theory Atom}
-    {Γ : Ctx Atom} {A : Proposition Atom} :
-    DerivableIn (T ∪ IPL : Theory Atom) (⟨Γ, A⟩ : Sequent) ↔
-    Nonempty (T.IntDerivation Γ A) := by
-  refine ⟨fun ⟨(D : (T ∪ IPL).Derivation Γ A)⟩ => ?_,
-    fun h => ⟨h.some.toDerivation⟩⟩
-  induction D with
-  | ax hA =>
-    cases hA
-    case inl hA => exact ⟨.ax hA⟩
-    case inr hA =>
-      obtain ⟨A, rfl⟩ := hA
-      exact ⟨.implI _ <| .efq A <| .ass (Finset.mem_insert_self ⊥ _)⟩
-  | ass hA => exact ⟨.ass hA⟩
-  | conjI DA DB aih bih => exact ⟨.conjI (aih ⟨DA⟩).some (bih ⟨DB⟩).some⟩
-  | conjE₁ D ih => exact ⟨.conjE₁ (ih ⟨D⟩).some⟩
-  | conjE₂ D ih => exact ⟨.conjE₂ (ih ⟨D⟩).some⟩
-  | disjI₁ D ih => exact ⟨.disjI₁ (ih ⟨D⟩).some⟩
-  | disjI₂ D ih => exact ⟨.disjI₂ (ih ⟨D⟩).some⟩
-  | disjE D DA DB ih aih bih => exact ⟨.disjE (ih ⟨D⟩).some (aih ⟨DA⟩).some (bih ⟨DB⟩).some⟩
-  | implI Γ D ih => exact ⟨.implI Γ (ih ⟨D⟩).some⟩
-  | implE D D' ih ih' => exact ⟨.implE (ih ⟨D⟩).some (ih' ⟨D'⟩).some⟩
+/-- Turnn a minimal derivation in the intuitionistic completion into an ordinary intuitionistic
+derivation. -/
+noncomputable def Theory.Derivation.toIDerivation {T : Theory Atom} {Γ : Ctx (WithBot Atom)}
+    {A : Proposition (WithBot Atom)} :
+    T.iCompletion.Derivation Γ A → T.toITheory.IDerivation Γ.toICtx A.toIProposition
+  | ax hA => by
+    by_cases hA' : A ∈ IPL (WithBot Atom)
+    · rw [←Classical.choose_spec hA']
+      exact .implI _ <| .efq _ <| .ass (Finset.mem_insert_self ..)
+    · apply ITheory.IDerivation.ax
+      obtain ⟨A', hAT, rfl⟩ : ∃ A' ∈ T, WithBot.some <$> A' = A := by
+        simpa [iCompletion, hA', Functor.map] using hA
+      use (discharger := rfl) A', hAT
+  | ass hA => ITheory.IDerivation.ass <| by simpa [Ctx.toICtx, Finset.mem_image] using ⟨A, hA, rfl⟩
+  | andI DA DB => DA.toIDerivation.conjI DB.toIDerivation
+  | andE₁ D => D.toIDerivation.conjE₁
+  | andE₂ D => D.toIDerivation.conjE₂
+  | orI₁ D => D.toIDerivation.disjI₁
+  | orI₂ D => D.toIDerivation.disjI₂
+  | orE D DA DB => D.toIDerivation.disjE
+    (Γ.toICtx_insert _ ▸ DA.toIDerivation) (Γ.toICtx_insert _ ▸ DB.toIDerivation)
+  | implI Γ D => (Γ.toICtx_insert _ ▸ D.toIDerivation).implI _
+  | implE D D' => D.toIDerivation.implE D'.toIDerivation
 
 end Cslib.Logic.PL
